extract page list to avoid circular dependencies

src/CallStack.v
@@ -1,13 +1,13 @@
 From RecordUpdate Require Import RecordSet.
 Import RecordSetNotations.
-Require Common Condition Ergs Memory Instruction CodeStorage.
+Require Common Condition Ergs Memory Pages.
 
-Import ZArith Condition Common Ergs MemoryBase Memory CodeStorage Instruction ZMod List ListNotations.
+Import ZArith Condition Common Ergs MemoryBase Memory Pages ZMod List ListNotations.
 
 Open Scope ZMod_scope.
 
 Definition CALLSTACK_LIMIT : nat := 1024.
-Definition page := page instruction_predicated instruction_invalid.
+(*Definition page := page instruction_predicated instruction_invalid. *)
 
 Definition exception_handler := code_address.
 
@@ -21,13 +21,40 @@ Record callframe_common := mk_cf {
   settable! mk_cf < cf_exception_handler_location; cf_sp; cf_pc; cf_ergs_remaining >.
 
 Record shards := mk_shards {
-      shard_this: shard_id;
-      shard_caller: shard_id;
-      shard_code: shard_id;
-  }.
+                     shard_this: shard_id;
+                     shard_caller: shard_id;
+                     shard_code: shard_id;
+                   }.
 
 #[export] Instance etaSH: Settable _ :=
   settable! mk_shards < shard_this; shard_caller; shard_code>.
+
+Record active_pages :=
+  mk_apages
+    {
+      ctx_code_page_id:  page_id;
+      ctx_const_page_id:  page_id;
+      ctx_stack_page_id:  page_id;
+      ctx_heap_page_id:  page_id;
+      ctx_auxheap_page_id:  page_id;
+      ctx_heap_bound: mem_address;
+      ctx_auxheap_bound: mem_address;
+    }.
+
+Definition list_active_pages (ap:active_pages) : list page_id :=
+  match ap with
+  | mk_apages code_id const_id stack_id heap_id auxheap_id _ _ =>
+      [code_id;const_id;stack_id;heap_id;auxheap_id]
+  end.
+
+Definition is_active_page (ap:active_pages) (id: page_id) : bool :=
+  List.existsb (Nat.eqb id) (list_active_pages ap).
+
+Definition page_older (id: page_id) (mps: active_pages) : bool :=
+  List.forallb (Nat.ltb id) (list_active_pages mps).
+
+#[export] Instance etaAP: Settable _ := settable! mk_apages< ctx_code_page_id; ctx_const_page_id; ctx_stack_page_id; ctx_heap_page_id; ctx_auxheap_page_id; ctx_heap_bound; ctx_auxheap_bound >.
+
 
 Record callframe_external :=
   mk_extcf {
@@ -53,14 +80,14 @@ Definition callstack := callframe.
 
 Fixpoint callframe_depth cf :=
   (match cf with
-| InternalCall x tail => 1 + callframe_depth tail
-| ExternalCall x (Some tail)=> 1 + callframe_depth tail
-| ExternalCall x None => 1
-end)%nat.
+   | InternalCall x tail => 1 + callframe_depth tail
+   | ExternalCall x (Some tail)=> 1 + callframe_depth tail
+   | ExternalCall x None => 1
+   end)%nat.
 
 Definition stack_overflow (xstack:callstack) : bool :=
   Nat.ltb CALLSTACK_LIMIT (callframe_depth xstack).
-                                                           
+
 Definition cfc (ef: callframe) : callframe_common :=
   match ef with
   | InternalCall x _ => x
@@ -73,235 +100,276 @@ Definition cfc_map (f:callframe_common->callframe_common) (ef: callframe) : call
   | ExternalCall x tail => ExternalCall (x <| ecf_common ::= f |>) tail
   end.
 
-Definition active_exception_handler (ef: callframe) : exception_handler :=
-  (cfc ef).(cf_exception_handler_location).
+
+  Section Ergs.
+
+    Definition ergs_remaining (ef:callframe) : ergs := (cfc ef).(cf_ergs_remaining).
+    Definition ergs_map (f: ergs->ergs) (ef:callframe) : callframe
+      := cfc_map (fun x => x <| cf_ergs_remaining ::= f |>) ef.
+    Definition ergs_set newergs := ergs_map (fun _ => newergs).
+
+    Inductive ergs_reimburse : ergs -> callframe -> callframe -> Prop :=
+    | er_reimburse: forall delta new_ergs ef ef',
+        delta + ergs_remaining ef = (new_ergs, false) ->
+        ef' = ergs_set new_ergs ef ->
+        ergs_reimburse delta ef ef'.
 
 
-Section Ergs.
+    Inductive ergs_reimburse_caller_and_drop : callframe -> callframe -> Prop
+      :=
+    |erc_internal: forall caller new_caller cf,
+        ergs_reimburse (ergs_remaining (InternalCall cf caller)) caller
+          new_caller ->
+        ergs_reimburse_caller_and_drop (InternalCall cf caller) new_caller
+    |erc_external: forall caller new_caller cf,
+        ergs_reimburse (ergs_remaining (ExternalCall cf (Some caller))) caller
+          new_caller ->
+        ergs_reimburse_caller_and_drop (ExternalCall cf (Some caller)) new_caller.
 
-  Definition ergs_remaining (ef:callframe) : ergs := (cfc ef).(cf_ergs_remaining).
-  Definition ergs_map (f: ergs->ergs) (ef:callframe) : callframe
-    := cfc_map (fun x => x <| cf_ergs_remaining ::= f |>) ef.
-  Definition ergs_set newergs := ergs_map (fun _ => newergs).
+    Definition ergs_reset := ergs_set zero32.
 
-  Inductive ergs_reimburse : ergs -> callframe -> callframe -> Prop :=
-  | er_reimburse: forall delta new_ergs ef ef',
-      delta + ergs_remaining ef = (new_ergs, false) ->
-      ef' = ergs_set new_ergs ef ->
-      ergs_reimburse delta ef ef'.
+    Definition affordable ef (e:ergs): bool :=
+      match ergs_remaining ef - e with
+      | (paid, false) => true
+      | (overflowed, true) => false
+      end.
 
-
-  Inductive ergs_reimburse_caller_and_drop : callframe -> callframe -> Prop
-    :=
-  |erc_internal: forall caller new_caller cf,
-      ergs_reimburse (ergs_remaining (InternalCall cf caller)) caller
-        new_caller ->
-      ergs_reimburse_caller_and_drop (InternalCall cf caller) new_caller
-  |erc_external: forall caller new_caller cf,
-      ergs_reimburse (ergs_remaining (ExternalCall cf (Some caller))) caller
-        new_caller ->
-      ergs_reimburse_caller_and_drop (ExternalCall cf (Some caller)) new_caller.
-
-  Definition ergs_reset := ergs_set zero32.
-
-  Definition affordable ef (e:ergs): bool :=
-    match ergs_remaining ef - e with
-    | (paid, false) => true
-    | (overflowed, true) => false
-    end.
-
-  Inductive pay : ergs -> callframe -> callframe -> Prop :=
-  | pay_ergs : forall e ef paid,
-      ergs_remaining ef - e = (paid, false) ->
-      pay e ef (ergs_set paid ef).
-End Ergs.
+    Inductive pay : ergs -> callframe -> callframe -> Prop :=
+    | pay_ergs : forall e ef paid,
+        ergs_remaining ef - e = (paid, false) ->
+        pay e ef (ergs_set paid ef).
+  End Ergs.
 
 
-Section SP.
-  (** Fetching value of the stack pointer itself. *)
-  Definition sp_get (cf: callframe) : stack_address :=
-    (cfc cf).(cf_sp).
+  Section SP.
+    (** Fetching value of the stack pointer itself. *)
+    Definition sp_get (cf: callframe) : stack_address :=
+      (cfc cf).(cf_sp).
 
-  Definition sp_mod_extcall (f:stack_address->stack_address) ef :=
-    (ef <| ecf_common ::= fun cf => cf <| cf_sp ::=  f |> |>).
+    Definition sp_mod_extcall (f:stack_address->stack_address) ef :=
+      (ef <| ecf_common ::= fun cf => cf <| cf_sp ::=  f |> |>).
 
-  Inductive sp_mod_extcall_spec f: callframe_external -> callframe_external -> Prop :=
-  | sme_apply: forall a b c d e g h eh sp pc ss ergs,
-      sp_mod_extcall_spec f (mk_extcf a b c d e g h ss (mk_cf eh sp pc ergs))
-        (mk_extcf a b c d e g h ss (mk_cf eh (f sp) pc ergs)).
+    Inductive sp_mod_extcall_spec f: callframe_external -> callframe_external -> Prop :=
+    | sme_apply: forall a b c d e g h eh sp pc ss ergs,
+        sp_mod_extcall_spec f (mk_extcf a b c d e g h ss (mk_cf eh sp pc ergs))
+          (mk_extcf a b c d e g h ss (mk_cf eh (f sp) pc ergs)).
 
-  Theorem sp_mod_extcall_correct:
-    forall f ef, sp_mod_extcall_spec f ef (sp_mod_extcall f ef).
-  Proof.
-    intros f [].
-    destruct ecf_common0.
-    constructor.
-  Qed.
+    Theorem sp_mod_extcall_correct:
+      forall f ef, sp_mod_extcall_spec f ef (sp_mod_extcall f ef).
+    Proof.
+      intros f [].
+      destruct ecf_common0.
+      constructor.
+    Qed.
 
-  Definition sp_mod (f:stack_address->stack_address) ef : callframe :=
-    match ef with
-    | InternalCall x tail => InternalCall (x <| cf_sp ::=  f |>) tail
-    | ExternalCall x tail => ExternalCall (sp_mod_extcall f x) tail
-    end.
+    Definition sp_mod (f:stack_address->stack_address) ef : callframe :=
+      match ef with
+      | InternalCall x tail => InternalCall (x <| cf_sp ::=  f |>) tail
+      | ExternalCall x tail => ExternalCall (sp_mod_extcall f x) tail
+      end.
 
-  Definition sp_update new_sp := sp_mod (fun _ => new_sp).
+    Definition sp_update new_sp := sp_mod (fun _ => new_sp).
 
-  Inductive sp_mod_spec f : callframe -> callframe -> Prop :=
-  | usp_ext:
-    forall ecf ecf' tail,
-      sp_mod_extcall_spec f ecf ecf' ->
-      sp_mod_spec f (ExternalCall ecf tail) (ExternalCall ecf' tail)
-  | usp_int:
-    forall  eh sp pc ergs tail,
-      sp_mod_spec f (InternalCall (mk_cf eh sp pc ergs) tail) (InternalCall (mk_cf eh (f sp) pc ergs) tail).
+    Inductive sp_mod_spec f : callframe -> callframe -> Prop :=
+    | usp_ext:
+      forall ecf ecf' tail,
+        sp_mod_extcall_spec f ecf ecf' ->
+        sp_mod_spec f (ExternalCall ecf tail) (ExternalCall ecf' tail)
+    | usp_int:
+      forall  eh sp pc ergs tail,
+        sp_mod_spec f (InternalCall (mk_cf eh sp pc ergs) tail) (InternalCall (mk_cf eh (f sp) pc ergs) tail).
 
-  Theorem sp_mod_spec_correct f:
-    forall ef, sp_mod_spec f ef (sp_mod f ef).
-  Proof.
-    destruct ef; destruct c; constructor.
-    apply sp_mod_extcall_correct.
-  Qed.
+    Theorem sp_mod_spec_correct f:
+      forall ef, sp_mod_spec f ef (sp_mod f ef).
+    Proof.
+      destruct ef; destruct c; constructor.
+      apply sp_mod_extcall_correct.
+    Qed.
 
-End SP.
+  End SP.
 
 
-Section PC.
-  Definition pc_get (ef: callframe) : code_address :=
-    match ef with
-    | InternalCall cf _ => cf.(cf_pc)
-    | ExternalCall ef tail => ef.(ecf_common).(cf_pc)
-    end.
+  Section PC.
+    Definition pc_get (ef: callframe) : code_address :=
+      match ef with
+      | InternalCall cf _ => cf.(cf_pc)
+      | ExternalCall ef tail => ef.(ecf_common).(cf_pc)
+      end.
 
-  Definition pc_mod f ef :=
-    match ef with
-    | InternalCall x tail => InternalCall (x <| cf_pc ::=  f |>) tail
-    | ExternalCall x tail => ExternalCall (x <| ecf_common ::= fun cf => cf <| cf_pc ::=  f |> |>) tail
-    end.
+    Definition pc_mod f ef :=
+      match ef with
+      | InternalCall x tail => InternalCall (x <| cf_pc ::=  f |>) tail
+      | ExternalCall x tail => ExternalCall (x <| ecf_common ::= fun cf => cf <| cf_pc ::=  f |> |>) tail
+      end.
 
 
 
-  Definition pc_inc (pc pc':code_address) := uinc_overflow _ pc = (pc',false).
-  Definition pc_set new := pc_mod (fun _ => new).
+    Definition pc_inc (pc pc':code_address) := uinc_overflow _ pc = (pc',false).
+    Definition pc_set new := pc_mod (fun _ => new).
 
-  Inductive update_pc_cfc : code_address -> callframe_common -> callframe_common
-                            -> Prop :=
-  | uupdate_pc:
-    forall ehl sp ergs pc pc',
-      update_pc_cfc pc' (mk_cf ehl sp pc ergs) (mk_cf ehl sp pc' ergs).
+    Inductive update_pc_cfc : code_address -> callframe_common -> callframe_common
+                              -> Prop :=
+    | uupdate_pc:
+      forall ehl sp ergs pc pc',
+        update_pc_cfc pc' (mk_cf ehl sp pc ergs) (mk_cf ehl sp pc' ergs).
 
-  Inductive update_pc_extcall: code_address -> callframe_external -> callframe_external
-                               -> Prop :=
-  | upe_update:
-    forall pc' cf cf' this_address msg_sender code_address pages is_static context_u128_value saved_storage_state ss,
-      update_pc_cfc pc' cf cf' ->
-      update_pc_extcall pc'
-        (mk_extcf this_address msg_sender code_address pages is_static
-           context_u128_value saved_storage_state ss cf)
-        (mk_extcf this_address msg_sender code_address pages is_static
-           context_u128_value saved_storage_state ss cf')
-  .
+    Inductive update_pc_extcall: code_address -> callframe_external -> callframe_external
+                                 -> Prop :=
+    | upe_update:
+      forall pc' cf cf' this_address msg_sender code_address pages is_static context_u128_value saved_storage_state ss,
+        update_pc_cfc pc' cf cf' ->
+        update_pc_extcall pc'
+          (mk_extcf this_address msg_sender code_address pages is_static
+             context_u128_value saved_storage_state ss cf)
+          (mk_extcf this_address msg_sender code_address pages is_static
+             context_u128_value saved_storage_state ss cf')
+    .
 
-  Inductive update_pc : code_address -> callframe -> callframe -> Prop :=
-  | upc_ext:
-    forall ecf ecf' tail pc',
-      update_pc_extcall pc' ecf ecf' ->
-      update_pc pc' (ExternalCall ecf tail) (ExternalCall ecf' tail)
-  | upc_int:
-    forall pc' cf cf' tail,
-      update_pc_cfc pc' cf cf' ->
-      update_pc pc' (InternalCall cf tail) (InternalCall cf' tail).
+    Inductive update_pc : code_address -> callframe -> callframe -> Prop :=
+    | upc_ext:
+      forall ecf ecf' tail pc',
+        update_pc_extcall pc' ecf ecf' ->
+        update_pc pc' (ExternalCall ecf tail) (ExternalCall ecf' tail)
+    | upc_int:
+      forall pc' cf cf' tail,
+        update_pc_cfc pc' cf cf' ->
+        update_pc pc' (InternalCall cf tail) (InternalCall cf' tail).
 
-  Theorem update_pc_correct:
-    forall ef pc, update_pc pc ef (pc_set pc ef).
-  Proof.
-    intros [ []|[] ] pc; simpl; [|destruct ecf_common0]; repeat constructor.
-  Qed.
+    Theorem update_pc_correct:
+      forall ef pc, update_pc pc ef (pc_set pc ef).
+    Proof.
+      intros [ []|[] ] pc; simpl; [|destruct ecf_common0]; repeat constructor.
+    Qed.
 
-End PC.
+  End PC.
 
-Section TopmostExternalFrame.
+  Section TopmostExternalFrame.
 
-  Fixpoint topmost_extframe (ef : callframe) : callframe_external :=
-    match ef with
-    | InternalCall _ tail => topmost_extframe tail
-    | ExternalCall x tail => x
-    end.
+    Fixpoint topmost_extframe (ef : callframe) : callframe_external :=
+      match ef with
+      | InternalCall _ tail => topmost_extframe tail
+      | ExternalCall x tail => x
+      end.
 
-  Inductive topmost_extframe_spec : callframe -> callframe_external -> Prop :=
-  | te_Top: forall x t, topmost_extframe_spec (ExternalCall x t) x
-  | te_Deeper: forall c t f,
-      topmost_extframe_spec t f -> topmost_extframe_spec (InternalCall c t) f
-  .
-  Theorem topmost_extframe_correct:
-    forall ef, topmost_extframe_spec ef (topmost_extframe ef).
-  Proof.
-    induction ef; constructor; auto.
-  Qed.
-
-
-  Fixpoint change_topmost_extframe f (ef:callframe) : callframe :=
-    match ef with
-    | InternalCall x tail => InternalCall x (change_topmost_extframe f tail)
-    | ExternalCall x tail => ExternalCall (f x) tail
-    end.
-
-  Inductive change_topmost_extframe_spec f : callframe -> callframe -> Prop :=
-  | ct_base: forall cf t,
-      change_topmost_extframe_spec f (ExternalCall cf t) (ExternalCall (f cf) t)
-  | ct_ind: forall cf t t',
-      change_topmost_extframe_spec f t t' ->
-      change_topmost_extframe_spec f (InternalCall cf t) (InternalCall cf t')
-  .
-
-  Lemma change_topmost_extframe_correct : forall f ef,
-      change_topmost_extframe_spec f ef (change_topmost_extframe f ef).
-  Proof.
-    intros f ef.
-    induction ef as [x tail | x tail]; simpl.
-    - apply ct_ind; apply IHtail.
-    - simpl.
-      apply ct_base.
-  Qed.
-
-  Definition update_memory_context (ctx:active_pages): callframe -> callframe :=
-    change_topmost_extframe (fun ef => ef <| ecf_pages := ctx |> ).
-
-End TopmostExternalFrame.
+    Inductive topmost_extframe_spec : callframe -> callframe_external -> Prop :=
+    | te_Top: forall x t, topmost_extframe_spec (ExternalCall x t) x
+    | te_Deeper: forall c t f,
+        topmost_extframe_spec t f -> topmost_extframe_spec (InternalCall c t) f
+    .
+    Theorem topmost_extframe_correct:
+      forall ef, topmost_extframe_spec ef (topmost_extframe ef).
+    Proof.
+      induction ef; constructor; auto.
+    Qed.
 
 
-Section ActivePages.
-  Definition get_active_pages (ef: callframe) : active_pages :=
-    (topmost_extframe ef).(ecf_pages).
+    Fixpoint change_topmost_extframe f (ef:callframe) : callframe :=
+      match ef with
+      | InternalCall x tail => InternalCall x (change_topmost_extframe f tail)
+      | ExternalCall x tail => ExternalCall (f x) tail
+      end.
 
-  Definition active_code_id (ef: callframe) : page_id :=
-    (get_active_pages ef).(ctx_code_page_id).
+    Inductive change_topmost_extframe_spec f : callframe -> callframe -> Prop :=
+    | ct_base: forall cf t,
+        change_topmost_extframe_spec f (ExternalCall cf t) (ExternalCall (f cf) t)
+    | ct_ind: forall cf t t',
+        change_topmost_extframe_spec f t t' ->
+        change_topmost_extframe_spec f (InternalCall cf t) (InternalCall cf t')
+    .
 
-  Definition active_stack_id (ef: callframe) : page_id :=
-    (get_active_pages ef).(ctx_stack_page_id).
+    Lemma change_topmost_extframe_correct : forall f ef,
+        change_topmost_extframe_spec f ef (change_topmost_extframe f ef).
+    Proof.
+      intros f ef.
+      induction ef as [x tail | x tail]; simpl.
+      - apply ct_ind; apply IHtail.
+      - simpl.
+        apply ct_base.
+    Qed.
 
-  Definition active_const_id (ef: callframe) : page_id :=
-    (get_active_pages ef).(ctx_const_page_id).
+    Definition update_memory_context (ctx:active_pages): callframe -> callframe :=
+      change_topmost_extframe (fun ef => ef <| ecf_pages := ctx |> ).
 
-  Definition active_heap_id (ef: callframe) : page_id :=
-    (get_active_pages ef).(ctx_heap_page_id).
-
-  Definition active_auxheap_id (ef: callframe) : page_id :=
-    (get_active_pages ef).(ctx_auxheap_page_id).
-
-  Definition heap_bound xstack := (get_active_pages xstack).(ctx_heap_bound).
-  Definition auxheap_bound xstack := (get_active_pages xstack).(ctx_auxheap_bound).
+  End TopmostExternalFrame.
 
 
-  Definition heap_variant_id (page_type: data_page_type)
-    :  callframe -> page_id :=
-    match page_type with
-    | Heap => active_heap_id
-    | AuxHeap => active_auxheap_id
-    end.
+  Section ActivePages.
+    Definition get_active_pages (ef: callframe) : active_pages :=
+      (topmost_extframe ef).(ecf_pages).
 
-  Definition heap_variant_bound (type:data_page_type):  callstack -> mem_address :=
-    match type with
-    | Heap => heap_bound
-    | AuxHeap => auxheap_bound
-    end.
-End ActivePages.
+    Definition active_code_id (ef: callframe) : page_id :=
+      (get_active_pages ef).(ctx_code_page_id).
+
+    Definition active_stack_id (ef: callframe) : page_id :=
+      (get_active_pages ef).(ctx_stack_page_id).
+
+    Definition active_const_id (ef: callframe) : page_id :=
+      (get_active_pages ef).(ctx_const_page_id).
+
+    Definition active_heap_id (ef: callframe) : page_id :=
+      (get_active_pages ef).(ctx_heap_page_id).
+
+    Definition active_auxheap_id (ef: callframe) : page_id :=
+      (get_active_pages ef).(ctx_auxheap_page_id).
+
+    Definition heap_bound xstack := (get_active_pages xstack).(ctx_heap_bound).
+    Definition auxheap_bound xstack := (get_active_pages xstack).(ctx_auxheap_bound).
+
+
+    Definition heap_variant_id (page_type: data_page_type)
+      :  callframe -> page_id :=
+      match page_type with
+      | Heap => active_heap_id
+      | AuxHeap => active_auxheap_id
+      end.
+
+    Definition heap_variant_bound (type:data_page_type):  callstack -> mem_address :=
+      match type with
+      | Heap => heap_bound
+      | AuxHeap => auxheap_bound
+      end.
+
+    Context {instruction:Type} (invalid: instruction).
+    Let pages := pages invalid.
+    Let page := page invalid.
+    Let page_has_id := page_has_id invalid.
+    
+    Definition active_exception_handler (ef: callframe) : exception_handler :=
+      (cfc ef).(cf_exception_handler_location).
+    
+    Inductive active_codepage : pages -> callframe -> page -> Prop :=
+    | ap_active_code: forall mm ef codepage,
+        page_has_id mm (active_code_id ef) codepage ->
+        active_codepage mm ef codepage.
+    
+    Inductive active_constpage : pages -> callframe -> page -> Prop :=
+    | ap_active_const: forall mm ef constpage,
+        page_has_id  mm (active_const_id ef) constpage ->
+        active_constpage mm ef constpage.
+
+    Inductive active_stackpage : pages -> callframe -> page -> Prop :=
+    | ap_active_stack: forall mm ef stackpage,
+        page_has_id mm (active_stack_id ef) stackpage ->
+        active_stackpage mm ef stackpage.
+
+    Inductive active_heappage : pages -> callframe -> page -> Prop :=
+    | ap_active_heap: forall mm ef heappage,
+        page_has_id mm (active_heap_id ef) heappage ->
+        active_heappage mm ef heappage.
+
+    Inductive active_auxheappage : pages -> callframe -> page -> Prop :=
+    | ap_active_auxheap: forall mm ef auxheappage,
+        page_has_id mm (active_auxheap_id ef) auxheappage ->
+        active_auxheappage mm ef auxheappage.
+
+    Definition heap_variant_page (page_type: data_page_type)
+      : pages -> callframe -> page -> Prop :=
+      match page_type with
+      | Heap => active_heappage
+      | AuxHeap => active_auxheappage
+      end.
+    Definition current_shard xstack : shard_id := (topmost_extframe xstack).(ecf_shards).(shard_this).
+
+    Definition current_contract xstack : contract_address := (topmost_extframe xstack).(ecf_this_address).
+    
+  End ActivePages.
