src/State.v
@@ -1,75 +1,19 @@
 From RecordUpdate Require Import RecordSet.
-Require Common Condition Ergs Memory Instruction CodeStorage CallStack.
+Require Common Ergs Memory Instruction CallStack CodeStorage Pages.
 
-Import ZArith Condition Common Ergs CallStack MemoryBase Memory CodeStorage Instruction ZMod List.
+Import ZArith Condition Common CodeStorage Ergs CallStack MemoryBase Memory Instruction Pages ZMod List.
 Import ListNotations RecordSetNotations.
 
-Definition page := page instruction_predicated instruction_invalid.
-Definition code_manager := code_manager instruction_predicated instruction_invalid.
+
+Definition page := page instruction_invalid.
+Definition pages := pages instruction_invalid.
+Definition code_manager := code_manager instruction_invalid.
 
 Definition exception_handler := code_address.
 
 Definition KERNEL_MODE_MAXADDR : contract_address := int_mod_of _ (2^16-1).
 
 
-Section AllocatedPages.
-  Import Bool Nat.
-
-  Definition pages : Type := list (page_id * page).
-
-  Inductive page_replace:  page_id -> page -> pages -> pages -> Prop :=
-  | mm_replace_base: forall oldpage id newpage tail,
-      page_replace id newpage ((id, oldpage)::tail) ((id,newpage)::tail)
-  | mm_replace_ind: forall oldpage id not_id newpage tail tail',
-      page_replace id newpage tail tail' ->
-      id <> not_id ->
-      page_replace id newpage ((not_id,oldpage)::tail) ((not_id,oldpage)::tail').
-
-  Inductive page_has_id : pages -> page_id -> page -> Prop :=
-  | mpid_select : forall mm id page,
-      List.In (id, page) mm ->
-      page_has_id mm id page.
-
-  Definition is_active_page (ef:callframe) (id: page_id) : bool :=
-    eqb (active_code_id ef) id ||
-      eqb (active_stack_id ef) id ||
-      eqb (active_const_id ef) id ||
-      eqb (active_heap_id ef) id ||
-      eqb (active_auxheap_id ef) id .
-
-    Inductive active_codepage : pages -> callframe -> page -> Prop :=
-    | ap_active_code: forall mm ef codepage,
-        page_has_id mm (active_code_id ef) codepage ->
-        active_codepage mm ef codepage.
-
-    Inductive active_constpage : pages -> callframe -> page -> Prop :=
-    | ap_active_const: forall mm ef constpage,
-        page_has_id mm (active_const_id ef) constpage ->
-        active_constpage mm ef constpage.
-
-    Inductive active_stackpage : pages -> callframe -> page -> Prop :=
-    | ap_active_stack: forall mm ef stackpage,
-        page_has_id mm (active_stack_id ef) stackpage ->
-        active_stackpage mm ef stackpage.
-
-    Inductive active_heappage : pages -> callframe -> page -> Prop :=
-    | ap_active_heap: forall mm ef heappage,
-        page_has_id mm (active_heap_id ef) heappage ->
-        active_heappage mm ef heappage.
-
-    Inductive active_auxheappage : pages -> callframe -> page -> Prop :=
-    | ap_active_auxheap: forall mm ef auxheappage,
-        page_has_id mm (active_auxheap_id ef) auxheappage ->
-        active_auxheappage mm ef auxheappage.
-
-  Definition heap_variant_page (page_type: data_page_type)
-    : pages -> callframe -> page -> Prop :=
-    match page_type with
-    | Heap => active_heappage
-    | AuxHeap => active_auxheappage
-    end.
-
-End AllocatedPages.
 
 
 Definition update_active_pages (ps:active_pages): callframe -> callframe :=
