src/CodeStorage.v
@@ -1,6 +1,6 @@
-Require Common Memory ABI lib.Decidability Log VersionedHash.
+Require Common ABI lib.Decidability Log MemoryOps VersionedHash.
 
-Import Log VersionedHash Common Decidability Ergs Memory MemoryBase ZArith ZMod ABI.
+Import Log VersionedHash Common Decidability Ergs MemoryOps Memory MemoryBase ZArith ZMod ABI.
 (** A separate code storage. It is an abstraction, because in the current *)
 (** implementation it is a part of a decommitter. *)
 
@@ -8,10 +8,9 @@ Definition DEPLOYER_SYSTEM_CONTRACT_ADDRESS : contract_address
   := (ZMod.int_mod_of _ (2^15))%Z.
 
 Section Defs.
-  Variable ins_type: Type.
-  Variable invalid_ins: ins_type.
+  Context {ins_type: Type} (invalid_ins: ins_type).
 
-  Let code_page := code_page ins_type invalid_ins.
+  Let code_page := code_page invalid_ins.
 
   Definition code_storage_params := {|
                                      addressable_block := code_page;
@@ -31,33 +30,36 @@ Section Defs.
 
   Definition is_fresh cm vh := negb (contains _ VersionedHash.eq_dec (cm_fresh cm) vh).
 
-  Inductive code_fetch_no_masking: shard -> code_storage
-                        -> contract_address -> (versioned_hash * code_page * code_length) -> Prop :=
-  | cfnm_load : forall (contracts:shard) (called_address:contract_address) deployer_storage hash_enc (code_storage:code_storage) code_length_in_words extra_marker partial_hash page_init,
-      load_result _ DEPLOYER_SYSTEM_CONTRACT_ADDRESS contracts deployer_storage ->
-      load_result storage_params (@resize _ 256 called_address) deployer_storage hash_enc ->
+  Definition code_hash_location (for_contract: contract_address) (sid:shard_id): fqa_key :=
+      mk_fqa_key sid DEPLOYER_SYSTEM_CONTRACT_ADDRESS (resize _ 256 for_contract).
+  
+  Inductive code_fetch_hash (d:depot) (cs: code_storage) (sid: shard_id) (contract_addr: contract_address) :
+   option (versioned_hash * code_length) -> Prop :=
+ |cfh_found: forall hash_enc code_length_in_words extra_marker partial_hash,
+      storage_read d (code_hash_location contract_addr sid) hash_enc ->
       hash_enc <> zero256 ->
-      hash_coder.(decode) hash_enc = Some (mk_vhash code_length_in_words extra_marker partial_hash) ->
       marker_valid extra_marker = true ->
-      load_result (code_storage_params) (@resize _ 256 partial_hash) code_storage page_init ->
-      code_fetch_no_masking contracts code_storage called_address ((mk_vhash code_length_in_words extra_marker partial_hash), page_init,code_length_in_words).
+      hash_coder.(decode) hash_enc = Some (mk_vhash code_length_in_words extra_marker partial_hash) ->
+      code_fetch_hash d cs sid contract_addr (Some (mk_vhash code_length_in_words extra_marker partial_hash, code_length_in_words))
 
-  Inductive code_fetch_shard: bool -> shard -> code_storage -> contract_address -> (versioned_hash * code_page * code_length) -> Prop :=
-  | cfh_load is_masking_allowed: forall (contracts:shard) (called_address:contract_address) (code_storage:code_storage) code_length_in_words extra_marker partial_hash page_init,
-      code_fetch_no_masking contracts code_storage called_address ((mk_vhash code_length_in_words extra_marker partial_hash), page_init,code_length_in_words) ->
-      code_fetch_shard is_masking_allowed contracts code_storage called_address ((mk_vhash code_length_in_words extra_marker partial_hash), page_init,code_length_in_words)
+  | cfh_not_found:
+      storage_read d (code_hash_location contract_addr sid) zero256 ->
+      code_fetch_hash d cs sid contract_addr None.
+                        
+  
+  Inductive code_fetch  (d:depot) (cs: code_storage) (sid: shard_id) (contract_addr: contract_address) :
+    bool -> (versioned_hash * code_page * code_length) -> Prop :=
+  | cfnm_no_masking: forall vhash (code_storage:code_storage) code_length_in_words page_init masking,
+      code_fetch_hash d cs sid contract_addr (Some (vhash, code_length_in_words)) ->
+      load_result code_storage_params (resize _ 256 (partial_hash vhash)) code_storage page_init ->
+      
+      code_fetch d cs sid contract_addr masking (vhash, page_init, code_length_in_words) 
+  | cfnm_masking: forall (code_storage:code_storage) code_length_in_words,
+      code_fetch_hash d cs sid contract_addr None ->
+      code_fetch d cs sid contract_addr true (DEFAULT_AA_VHASH, DEFAULT_AA_CODE _ invalid_ins,code_length_in_words).
 
-  | cfh_load_aa_default : forall (contracts:shard) (called_address:contract_address) deployer_storage (code_storage:code_storage),
-      load_result _ DEPLOYER_SYSTEM_CONTRACT_ADDRESS contracts deployer_storage ->
-      load_result storage_params (@resize _ 256 called_address) deployer_storage zero256->
-      code_fetch_shard true contracts code_storage called_address (DEFAULT_AA_VHASH, DEFAULT_AA_CODE _ invalid_ins,code_length_in_words DEFAULT_AA_VHASH).
-
-  Inductive code_fetch (depot:depot) (sid: shard_id): bool -> code_storage -> contract_address ->
-                                                      (versioned_hash * code_page * code_length) -> Prop :=
-| cfs_fetch: forall masking_allowed sh codes addr vh,
-    load_result _ sid depot sh ->
-    code_fetch_shard masking_allowed sh codes addr vh ->
-    code_fetch depot sid masking_allowed codes addr vh .
   
     
 End Defs.
+
+        
