src/Pages.v
@@ -1,0 +1,41 @@
+From RecordUpdate Require Import RecordSet.
+Require Common Memory lib.PMap_ext.
+Import Common Memory BinInt List PMap_ext.
+Import ListNotations.
+Import RecordSetNotations.
+
+Definition page_id := nat.
+
+Section Pages.
+  
+  Context {ins_type: Type} (inv: ins_type).
+  Inductive page :=
+  (** Heap or auxheap *)
+  | DataPage : data_page -> page
+  | StackPage : stack_page -> page
+  | ConstPage : const_page -> page
+  | CodePage : code_page inv -> page.
+
+  Inductive data_page_type := Heap | AuxHeap.
+
+  Definition pages := list (prod nat page).
+
+  Inductive page_has_id : pages -> page_id -> page -> Prop :=
+  | mpid_select : forall mm id page,
+      List.In (id, page) mm ->
+      page_has_id mm id page.
+
+  Inductive page_replace:  page_id -> page -> pages -> pages -> Prop :=
+  | mm_replace_base: forall oldpage id newpage tail,
+      page_replace id newpage ((id, oldpage)::tail) ((id,newpage)::tail)
+  | mm_replace_ind: forall oldpage id not_id newpage tail tail',
+      page_replace id newpage tail tail' ->
+      id <> not_id ->
+      page_replace id newpage ((not_id,oldpage)::tail) ((not_id,oldpage)::tail').
+
+
+  Definition page_alloc (p:page) (m: pages) : pages :=
+    cons (length m, p) m.
+
+
+End Pages.
